\documentclass[11pt,fleqn]{amsproc}
\usepackage{textcomp}

\newcommand{\R}{{\bf R}}
\newcommand{\F}{\mathcal{F}}
\newcommand{\G}{\mathcal{G}}
\renewcommand{\H}{\mathcal{H}}
\newcommand{\K}{\mathcal{K}}
\newcommand{\M}{\mathcal{M}}
\newcommand{\N}{\mathcal{N}}
\renewcommand{\P}{\mathcal{P}}
\newcommand{\X}{\mathcal{X}}

\newcommand{\Var}{\mathop{\rm{Var}}}
\newcommand{\Cov}{\mathop{\rm{Cov}}}
\renewcommand{\ker}{\mathop{\rm{ker}}}
\newcommand{\ran}{\mathop{\rm{ran}}}

%\newtheorem{prob}{Problem}[section]
%\newtheorem{cor}[thm]{Corollary}
\newtheorem{xca}{Exercise}

\renewcommand{\labelenumi}{(\alph{enumi})}

\begin{document}

\title{Derivative Securities Homework 7}
\author{Due 7:10PM, 4 April 2011}

\maketitle

\begin{xca}{(30 points)}
Consider the model with prices $X_j = (R_j, S_j, 0)$, $0\le j\le n$,
and cash flows $C_j = (0, 0, \Phi_j - \Phi_{j-1})$, $0 < j\le n$,
at times $t_0$, \dots, $t_n$, where $\Phi_n = S_n$.
Assume $\Pi_j$
is the no arbitrage price deflator.
Show $\Phi_j = E[\Phi_{j+1}\mid \F_j]$ if $\Pi_j$ is
$\F_{j-1}$ measurable. (We say $(\Pi_j)$ is {\em predictable}.)
Conclude $\Phi_0 = E[S_n]$.
\end{xca}

By the FTAP, $0 = E[(\Phi_j - \Phi_{j-1})\Pi_j\mid F_{j-1}]
= E[\Phi_j - \Phi_{j-1}\mid F_{j-1}]\Pi_j$
if $(\Pi_j)$ is predictable. We conclude
$\Phi_0 = E[\Phi_1] = \cdots E[\Phi_n] = E[S_n]$.

\begin{xca}{(30 points)}
Let $f = F(0;t,u)$ be the forward rate now and $F = F(t;t,u)$
be the forward rate expiration $t$ over the interval $[t,u]$.
From exercise 1, we know the futures rate at time zero is
$E[F]$. Find a formula for $E[F] - f$ involving $D_u$, the
stochastic discount to time $u$, and determine
under what conditions this difference is positive.
\end{xca}

Since the price of a forward contract is zero, we have
$0 = E[(F - f)D_u] = E[FD_u] - fE[D_u] = E[F]E[D_u] + \Cov(F,D_u)
- fE[D_u]$ so $E[F] - f = -\Cov(F,D_u)/D(0,u)$.  This is positive
if and only if $\Cov(F,D_u)$ is negative, which is usually the case.

\begin{xca}{(40 points)}
Consider the Ho-Lee short rate model $r_t = r + \sigma B_t$, where $r$
and $\sigma$ are constants and $B_t$ is standard Brownian motion.
\begin{enumerate}
\item Show $\int_s^t B_u\,du = tB_t - sB_s - \int_s^t u\,dB_u$.
\item Using the fact $e^{-\int_0^t\theta(u)\,dB_u - \int_0^t\theta^2(u)/2\,du}$
is a martingale, find a closed form formula for
$D(s,t) = E[D_t/D_s|\F_s]$ where $D_t = e^{-\int_0^t r_u\,du}$ is
the stochastic discount.
\end{enumerate}
\end{xca}

Lets do the general case $r_t = r(t) + \sigma(t) B_t$.
By Ito's formula, $d(\theta(t)B_t) = \theta(t)\,dB_t + \theta'(t)B_t\,dt$.
Let $\Sigma(t) = \int_0^t \sigma(s)\,ds$. We have
\begin{eqnarray*}
D(s,t) &=&
E[e^{-\int_s^t r_u\,du}\mid\F_s]\\
&=& E[e^{-\int_s^t (r(u) + \sigma(u)B_u)\,du}\,du\mid\F_s]\\
&=& e^{-\int_s^t r(u)\,du}E[e^{-\int_s^t \sigma(u)B_u}\,du\mid\F_s].\\
\end{eqnarray*}
Now
\begin{eqnarray*}
E[e^{-\int_s^t \sigma(u)B_u}\,du\mid\F_s] 
&=& E[e^{-\Sigma(t)B_t + \Sigma(s)B_s
	+\int_s^t \Sigma(u)\,dB_u}\mid\F_s]\\
&=& e^{-(\Sigma(t) - \Sigma(s))B_s}
	E[e^{-\Sigma(t)B_t + \Sigma(t)B_s
	+\int_s^t \Sigma(u)\,dB_u}\mid\F_s]\\
&=& e^{-(\Sigma(t) - \Sigma(s))B_s}
	E[e^{-\int_s^t (\Sigma(u) - \Sigma(t))\,dB_u}\mid\F_s]\\
&=& e^{-(\Sigma(t) - \Sigma(s))B_s}
	e^{+\int_s^t (\Sigma(u) - \Sigma(t))^2/2\,du}\\
\end{eqnarray*}
Putting it back together gives the general formula
\begin{eqnarray*}
D(s,t)
&=& e^{-\int_s^t r(u) - (\Sigma(u) - \Sigma(t))^2/2\,du
-(\Sigma(t) - \Sigma(s))B_s}\\
\end{eqnarray*}

For constant $r$ and $\sigma$, $\Sigma(t) = \sigma t$ so
\begin{eqnarray*}
D(s,t)
&=& e^{-r(t - s) + \sigma^2(t - s)^3/6 - \sigma(t - s)B_s}\\
\end{eqnarray*}

\end{document}
