\documentclass[10pt,letterpaper,fleqn]{report}
\usepackage[utf8]{inputenc}
\usepackage{amsmath}
\usepackage{amsfonts}
\usepackage{amssymb}
\usepackage{lmodern}
\usepackage{kpfonts}
\usepackage{lmodern}
\usepackage[T1]{fontenc}

\author{Keith Lewis}
\title{Ho-Lee Model}
\begin{document}
\maketitle
Let the {\em short rate} be \(R_t = \phi(t) + \sigma(t)B_t\) where
\(B_t\) is Brownian motion. Define the {\em stochastic discount}
\(D_t = \exp(-\int_0^t R_s\,ds)\). The price at time \(t\) of a {zero
coupon bond} maturing at \(u\) is
\begin{align*}
D(t,u) &= E_t e^{-\int_t^u R_s\,ds}\\
	&= E_t e^{-\int_t^u \phi(s)\,ds}e^{-\int_t^u \sigma(s)B_s\,ds}.\\
\end{align*}
Using \(d(\Sigma B) = \Sigma dB + \Sigma' B\,ds\)  and
\(\exp(-\frac{1}{2}\int_0^t \theta^2\,ds + \int_0^t \theta\,dB_s)\) is
a martingale
\begin{align*}
D(t,u) e^{\int_t^u \phi(s)\,ds}
&= E_t e^{-(\Sigma(u)B_u - \Sigma(t)B_t) + \int_t^u \Sigma(s)\,dB_s}\\
&= E_t e^{-(\Sigma(u)B_u -\Sigma(u)B_t + \Sigma(u)B_t - \Sigma(t)B_t) + \int_t^u \Sigma(s)\,dB_s}\\
&= E_t e^{-(\Sigma(u) - \Sigma(t))B_t + \int_t^u \Sigma(s) - \Sigma(u)\,dB_s}\\
&= e^{-(\Sigma(u) - \Sigma(t))B_t + \frac{1}{2}\int_t^u (\Sigma(s) - \Sigma(u))^2\,ds}\\
\end{align*}
hence
\[
D(t,u) = e^{-\int_t^u \phi(s) 
- \frac{1}{2}(\Sigma(u) - \Sigma(s))^2\,ds
- (\Sigma(u) - \Sigma(t))B_t}.
\]
Let \(\Phi(u,v)\) denote the integral and
\(\Delta(u,v)\) the coefficient of \(B_t\).

Recall the forward rate at time \(t\) over the interval \([u,v]\) having
daycount fraction \(\delta_{u,v}\) is
\[
F(t;u,v) = \frac{1}{\delta_{u,v}}\bigl(\frac{D(t,u)}{D(t,v)} - 1\bigr).
\]
In the Ho-Lee model \(F(t,u) = F(t;t,u) = (e^{\Phi(t,u) + \Delta(t,u)B_t} - 1)/\delta\)
the the payoff of a caplet is \(\max\{F(t,u)-k,0\}\delta = 
\max\{e^{\Phi + \Delta B_t} - 1 - \delta k, 0\}\) so it can be priced using
the Black-Scholes/Merton formula.

\section{Hull-White}
The short rate for the Hull-White model satisfies
\(dR = (\psi(t) - \alpha(t)R_t)\,dt + \sigma(t)\,dB_t\)
so \(dR - \alpha(t) R_t\,dt = \psi(t)\,dt + \sigma(t)\,dB_t\).
Using the integrating factor \(e^{-A(t)}\) where \(A'(t) = \alpha(t)\) gives
\[
e^{-A(t)}R_t - R_0 = \int_0^t e^{-A(s)}\psi(s)\,ds 
+ \int_0^t e^{-A(s)}\sigma(s)\,dB_s
\]
and so
\[
R_t = R_0 + \int_0^t e^{A(t)-A(s)}\psi(s)\,ds 
+ \int_0^t e^{A(t)-A(s)}\sigma(s)\,dB_s
\]
Note if \(\alpha = 0\) and \(\sigma\) is constant
this parameterization gives the Ho-Lee model with \(\psi = \phi'\).
We have
\begin{align*}
E_t e^{-\int_t^u R_s\,ds}&= e^{\Psi(t,u)}E_t e^{-\int_t^u\int_0^s\Sigma(v)\,dB_v\,ds}\\ 
&= e^{\Psi(t,u)}E_t e^{-\int_t^u(\int_0^t + \int_t^s)\Sigma(v)\,dB_v\,ds}\\ 
&= e^{\Psi(t,u)}E_t e^{-\int_0^t\int_t^u \Sigma(v)\,ds\,dB_v 
- \int_t^u\int_v^u\Sigma(v)\,ds\,dB_v}\\ 
&= e^{\Psi(t,u)}E_t e^{-(u - t)\int_0^t\Sigma(v)\,dB_v 
- \int_t^u(u - v)\Sigma(v)\,dB_v}\\ 
&= e^{\Psi(t,u)}e^{\frac{1}{2}(u - t)^2\int_0^t\Sigma(v)^2\,dv 
+ \frac{1}{2}\int_t^u(u - v)^2\Sigma(v)^2\,dv}\\ 
\end{align*}
\end{document}